Updated the different modules - most of them is now compilable
Updated gitignore
Added a Makefile and setenv.sh

Code/IdentityProvider.fst
@@ -6,40 +6,17 @@ open Crypto
 authentication method and then prompt client for it - and handle if the clients
 information was correct *)
 
-type SecurityRestriction = 
+(*type SecurityRestriction = 
 	| Session: 1
 	| User: 2
 	| IdP: 4
 
 type SecurityProfile =
 	| Profile:	prin -> SecurityRestriction ->
-				int -> SecurityProfile
-
-val identityprovider: me:prin -> user:prin -> authp:prin -> unit
+				int -> SecurityProfile*)
 val authenticateuser: me:prin -> user:prin -> authp:prin -> unit
 
-let rec identityprovider me user authp =
-	let request = ReceiveSaml user in
-	match request with
-	| Login (loginInfo) ->
-		(*let authnReq = CreateAuthnRequestMessage me authp in
-		assume(Log me authnReq);
-		let meprivk = CertStore.GetPrivateKey me in
-		let sigIdP = Sign me meprivk authnReq in
-		let response = AuthnRequestMessage me authp authnReq sigIdP in*)
-		(*sendsaml to authenticationprovider with logininfo*)
-		let authnReq = CreateAuthnRequestMessage me authp in
-		assume(Log me authnReq);
-		let myprivk = CertStore.GetPrivateKey me in
-		let sigIdP = Sign me myprivk authnReq in
-		let req = AuthnRequestMessage me authp authnReq loginInfo sigIdP in
-		SendSaml authp req;
-		identityprovider me user authp
-	| 
-	| _ -> SendSaml user (DisplayError 400);
-		identityprovider me user authp
-
-let rec authenticateuser me user authp =
+let authenticateuser me user authp =
 	let request = ReceiveSaml authp in
 	match request with
 	| AuthResponseMessage(issuer, destination, encassertion, authmethod) ->
@@ -51,9 +28,54 @@ let rec authenticateuser me user authp =
 			if VerifySignature authp pubkissuer token sigAuthP
 			then
 				(assert (Log authp token);
-				let response = UserAuthRequest authmethod request in
+				let response = UserAuthRequest authmethod in
 				SendSaml user response)
-			else SendSaml user (DisplayError 403);
-			authenticateuser me user authp
+			else SendSaml user (DisplayError 403)
+	| _ -> SendSaml user (DisplayError 400)
+
+val handlenfactorauth: auth:Authentication -> correctAuth:Authentication -> bool
+
+let handlenfactorauth auth correctAuth =
+	match auth with
+	| Facebook(id) -> true
+  	| SMS(useranswer) -> true
+  	| Google(id) -> true
+  	| OpenId(id) -> true
+  	| _ -> false
+
+
+val identityprovider: me:prin -> user:prin -> authp:prin -> unit
+
+let rec identityprovider me user authp =
+	let request = ReceiveSaml user in
+	match request with
+	| Login (loginInfo) ->
+		let authnReq = CreateAuthnRequestMessage me authp in
+		assume(Log me authnReq);
+		let myprivk = CertStore.GetPrivateKey me in
+		let sigIdP = Sign me myprivk authnReq in
+		let req = AuthnRequestMessage me authp authnReq loginInfo sigIdP in
+		SendSaml authp req;
+		authenticateuser me user authp;
+		identityprovider me user authp
+	| UserAuthenticated(status, logindata, authmethod) ->
+		match logindata with
+		| MkLoginData(user, sig, cert, auth, site, data) ->
+			if (status = "OK") && (VerifySignature user cert data sig) then
+				(assert (Log user data);
+					if handlenfactorauth auth authmethod then
+						let resp = LoginResponse "You are now logged in" in
+						SendSaml user resp;
+						identityprovider me user authp
+					else
+						let response = LoginResponse "Incorrect authentication" in
+						SendSaml user response;
+						identityprovider me user authp
+				)
+			else
+				SendSaml user (DisplayError 400);
+      			identityprovider me user authp
+      	| _ -> SendSaml user (DisplayError 400);
+      		identityprovider me user authp
 	| _ -> SendSaml user (DisplayError 400);
-		authenticateuser me user authp
+		identityprovider me user authp
