Code/Database.fst
@@ -25,7 +25,7 @@ val checkcprlogin: cpr:int -> password:string -> bool
 val checkuserlogin: user:string -> password:string -> bool
 
 val revokeidp: cpr:int -> idp:prin -> unit
-val revokeidp: user:string -> idp:prin -> unit
+val cprrevokeidp: user:string -> idp:prin -> unit
 
 val revokedidp: user:string -> idp:prin -> bool
 val cprrevokedidp: cpr:int -> idp:prin -> bool
